asychronous automata initial commit: just confirmed LHZ rule list

src/asynchronous_automata.lean
@@ -62,15 +62,16 @@ def equiv.on_prod {α α' β β'} (f : α ≃ α') (g : β ≃ β') : (α × β)
 
 } 
 
-def template.equiv_aux : (inside_outside × vonNeumann) ≃ fin 8 := 
+def template.read_aux : (inside_outside × vonNeumann) ≃ fin 8 := 
   equiv.trans (equiv.on_prod inside_outside.to_fin2 vonNeumann_fin4) fin.prod_equiv
 
-def template.equiv (α) : template α ≃ array (2*4) α := { 
-    to_fun := λ t, ⟨λ n, let p := (template.equiv_aux.inv_fun n) in t p.1 p.2 ⟩,
-    inv_fun := λ a i_o dir, a.data (template.equiv_aux (i_o, dir)),
-    left_inv := _,
-    right_inv := _ 
-  }
+structure template (α : Type) := (to_array : array (8) α)
+
+def template.read {α} (arr : template α) (io : inside_outside) (dir : vonNeumann) : α :=
+  arr.to_array.read (template.read_aux (io, dir))
+
+def template.from_fun {α} (f : inside_outside → vonNeumann → α) : template α :=
+  ⟨⟨λ ix, function.uncurry f (template.read_aux.inv_fun ix)⟩⟩
 
 def ACA_rule (α) := (template α → template α → Prop)
 
@@ -100,14 +101,159 @@ lemma vonNeumann.neg_involution (dir : vonNeumann) : -(-dir) = dir :=
   | W := rfl
   end
     
-def read_template (n m) (α : Type) 
+def read_template.aux {n m} {α : Type} 
   (mat : aMatrix (n+1) (m+1) (vonNeumann → α)) 
-  (ix : fin (n+1) × fin (m+1)) : 
-  template α
+  (ix : fin (n+1) × fin (m+1)) : inside_outside → vonNeumann → α
   | inside dir := (mat.read ix) dir
   | outside dir := 
     let offset : (fin (n+1) × fin (m+1)) := dir.to_index in
     mat.read (ix.1 + offset.1, ix.2 + offset.2) (-dir)
 
-def template.diff (α) : template α → template α → template Prop
-  | a b := functor.map (λ x y : α, x ≠ y) <$> a <*> b
+def read_template {n m} {α : Type} 
+  (mat : aMatrix (n+1) (m+1) (vonNeumann → α)) 
+  (ix : fin (n+1) × fin (m+1)) :
+  template α := template.from_fun (read_template.aux mat ix)
+
+instance : functor template := { 
+  map := λ α β f t, ⟨f <$> t.to_array⟩,
+  map_const := λ α β (f : α) t, ⟨f <$ t.to_array⟩
+}
+
+lemma template.map.def {α β} {f : α → β} {t : template α} : f <$> t = template.mk (f <$> t.to_array) := rfl
+
+lemma template.comp_map (α β γ : Type)
+  (f : α → β)
+  (g : β → γ)
+  (t : array 8 α) :
+  (g ∘ f) <$> t = g <$> f <$> t := by {
+  simp only, 
+  apply is_lawful_functor.comp_map
+}
+
+instance : is_lawful_functor template := {
+  id_map := λ α ⟨t⟩, by {have := id_map t, rw template.map.def, simp only, apply this},
+  comp_map := λ α β γ f g ⟨t⟩, by {have := comp_map f g t, simp_rw template.map.def, apply this},
+}
+
+def template.seq {α β : Type} : template (α → β) → template α → template β
+  | f x := template.mk (⟨λ ix, f.to_array.read ix $ x.to_array.read ix⟩)
+
+instance : applicative template := {
+  seq := λ _ _, template.seq ,
+  pure := λ α a, ⟨⟨λ _, a⟩⟩,
+}
+
+def bneq {α} [decidable_eq α] (x y : α) :=
+  if x ≠ y then tt else ff
+
+def template.hamming {α} [decidable_eq α] (a b: template α) : ℕ :=
+  (bneq <$> a <*> b).to_array.count id
+
+def aMatrix.hamming {α n m} [decidable_eq α] (a b: aMatrix n m α) : ℕ :=
+  array.count (⟨λ ix, bneq a.flattened b.flattened⟩ : array (n * m) bool) id
+
+def vonNeumann.decidable_eq.aux {α} [decidable_eq α] (f g : vonNeumann → α) : decidable (∀ x, f x = g x) :=
+  if h : f N = g N ∧ f E = g E ∧ f S = g S ∧ f W = g W
+    then is_true (by {rcases h with ⟨h_n, h_e, h_s, h_w⟩, intros x, cases x; assumption})
+    else is_false (λ all, h (by {simp_rw all, repeat {split; try {refl}}}))
+
+instance {α} [decidable_eq α] : decidable_eq (vonNeumann → α) :=
+  by {
+    intros a b,
+    have H : (a = b) ↔ (∀ nv, a nv = b nv) := by {split; intros h, {intros x, rw h}, funext, apply h},
+    rw H,
+    apply vonNeumann.decidable_eq.aux,
+  }
+
+structure ACA_step {α : Type} [decidable_eq α] (r : ACA_rule α) {n m} (a b : ACA_board (n+1) (m+1) α) :=
+   (ix : fin (n+1) × fin (m+1))
+   (t₀ t₁ : template α)
+   (r_t₀_t₁ : r t₀ t₁)
+   (a_matches_t₀ : read_template a ix = t₀)
+   (b_matches_t₁ : read_template b ix = t₁)
+   (no_other_difference : a.hamming b = t₀.hamming t₁)
+
+inductive path {α : Type} (r : α → α → Type) : α → α → Type
+  | refl : ∀ a, path a a
+  | snoc : ∀ a b c, path a b → r b c → path a c
+
+def weak_reachabable {α : Type} [decidable_eq α] (r : ACA_rule α) {n m} (a b : ACA_board (n+1) (m+1) α) :=
+  inhabited (path (ACA_step r) a b)
+
+def array.to_template (arr : array 8 (fin 2)) : template bool := ⟨arr.map (λ n, if n = 0 then tt else ff)⟩
+def array.last {α n} (arr : array (n+1) α) := arr.read (fin.last n)
+
+@[simp]
+lemma array.last_def {α n} (arr : array (n+1) α) : arr.last = arr.read (fin.last n) := rfl
+
+instance {α} [linear_order α] : linear_order (template α) := 
+  linear_order.preimage (by {
+    refine function.embedding.trans ⟨template.to_array, _⟩ ⟨array.to_list, _⟩; intros x y,
+    {
+      cases x; cases y,
+      simp only,
+      intro h; exact h,
+    },
+    {
+      intro inj_hyp,
+      transitivity x.to_list.to_array,
+      have H := (array.to_list_to_array x).symm,
+      apply H.elim, refl,
+      have H := (array.to_list_to_array y),
+      apply H.elim,
+      congr' 1,
+    }
+  })
+  
+def array.rev {α} {n} (arr : array (n+1) α) : array (n+1) α := ⟨λ ix, arr.read (fin.last n - ix)⟩
+
+notation `#[` arr:(foldr `,` (h t, array.push_back t h) array.nil `]`) := arr.rev
+
+def array.to_vector {n α} (arr : array n α) : vector α n := 
+  ⟨arr.to_list, array.to_list_length arr⟩ 
+
+def ACA_rules.from_list : list (array 2 (array 8 (fin 2))) →  rbmap (template bool) (template bool)
+  | l :=
+    let to_templates : array 2 (array 8 (fin 2)) → (template bool × template bool) :=
+      λ arr, 
+        match (arr.map array.to_template).to_vector with
+        | ⟨[old, new], _⟩ := ⟨old, new⟩
+        end
+      in
+    (l.map to_templates)
+
+def convert_from_dixons : array 8 (fin 2) → array 8 (fin 2)
+  | arr := 
+    match arr.to_vector with
+    | ⟨[i_top, i_bottom, i_left, i_right, o_top, o_bottom, o_left, o_right], p⟩ := -- T, B, L, R order
+      #[i_top, i_right, i_bottom, i_left, o_top, o_right, o_bottom, o_left] -- N, E, S, W order!
+    end
+
+def convert_from_dixons' : array 2 (array 8 (fin 2)) → array 2 (array 8 (fin 2))
+  | arr := arr.map convert_from_dixons
+
+def LHZ_list := 
+  list.map (λ arr, array.map arr convert_from_dixons)
+  [
+    #[#[0,0,0,0,0,0,1,0], #[0,0,0,1,0,0,0,0]], -- move forward
+    #[#[1,0,0,0,1,1,0,0], #[1,0,0,1,1,0,0,0]], -- Turn Left (head on)
+		#[#[0,0,1,0,0,1,1,0], #[0,0,1,1,0,0,1,0]], -- Turn Left (right side collison)
+		#[#[1,0,0,1,1,1,0,1], #[1,0,1,1,1,0,0,1]], -- Turn Right
+		#[#[0,0,1,1,0,1,1,1], #[1,1,0,1,1,1,0,0]]  -- Toggle Memory
+  ]
+
+def LHZ_base : rbmap (template bool) (template bool) :=
+  ACA_rules.from_list LHZ_list
+
+def template.print {α} (to_char : α → char) (t : template α) : string := 
+  match t.to_array.to_vector with
+  | ⟨[i_north, i_east, i_south, i_west, o_north, o_east, o_south, o_west], _⟩ :=
+    "\n  " ++ ⟨[to_char o_north]⟩ ++ "  \n" ++
+    "  " ++ ⟨[to_char i_north]⟩ ++ "  \n" ++
+    ⟨[to_char o_west, to_char i_west, ' ', to_char i_east, to_char o_east]⟩ ++ "\n" ++
+    "  " ++ ⟨[to_char i_south]⟩ ++ "  \n" ++
+    "  " ++ ⟨[to_char o_south]⟩ ++ "  \n"
+  end
+
+instance : has_to_string (template bool) := ⟨template.print (λ b, if b then '╬' else '█')⟩
+
